new/golang/defn/slice.v
@@ -76,11 +76,10 @@ Definition append t : val :=
   copy t (slice t "s_new" (len "s") (len "s_new")) "x" ;;
   "s_new".
 
-(* FIXME: this shouldn't take len as input *)
-(* Takes in a list of the specified length as input, and turns it into a
-   heap-allocated slice. *)
+(* Takes in a list as input, and turns it into a heap-allocated slice. *)
 Definition literal t : val :=
-  λ: "len" "elems",
+  λ: "elems",
+  let: "len" := list.Length "elems" in
   let: "s" := make2 t "len" in
   let: "l" := ref "elems" in
   let: "i" := ref_ty uint64T (zero_val uint64T) in
